matching-logic/src/ProofInfo.v
@@ -2,7 +2,7 @@ From Coq Require Import ssreflect ssrfun ssrbool.
 
 From Ltac2 Require Import Ltac2.
 
-From Coq Require Import Ensembles Bool String.
+From Coq Require Import Ensembles Bool String Btauto.
 From Coq.Logic Require Import FunctionalExtensionality Eqdep_dec.
 From Equations Require Import Equations.
 
@@ -30,7 +30,7 @@ Set Default Proof Mode "Classic".
 Open Scope ml_scope.
 
 (** For goals shaped like ProoInforMeeaning _ _ _ BasicReasoning *)
-Ltac solve_pim_simple := constructor; simpl;[(set_solver)|(set_solver)|(reflexivity)].
+Ltac solve_pim_simple := constructor; simpl;[(set_solver)|(set_solver)|(reflexivity)|(reflexivity)].
 
 
 Lemma useBasicReasoning {Σ : Signature} {Γ : Theory} {ϕ : Pattern} (i : ProofInfo) :
@@ -42,11 +42,15 @@ Proof.
   remember (proj1_sig H) as _H.
   exists (_H).
   clear Heq_H.
-  abstract (
-    destruct Hpf as [Hpf1 Hpf2 Hpf3];
+  destruct Hpf as [Hpf1 Hpf2 Hpf3 Hpf4].
   destruct i; constructor; simpl in *;
-  [set_solver|set_solver|idtac];
-  (destruct (uses_kt _H); simpl in *; try congruence)).
+  [set_solver|set_solver|idtac|idtac].
+  {
+    (destruct (uses_kt _H); simpl in *; try congruence).
+  }
+  {
+    (destruct (uses_kt_unreasonably _H); simpl in *; try congruence).
+  }
 Defined.
 
 
@@ -88,14 +92,44 @@ Proof.
     { apply H2. }
   }
   {
-    abstract(
+    
       simpl;
       destruct H1 as [pf1 Hpf1];
       destruct H2 as [pf2 Hpf2];
       destruct Hpf1,Hpf2;
       constructor; simpl;
-      [set_solver|set_solver|(destruct (uses_kt pf1),(uses_kt pf2); simpl in *; congruence)]
-    ).
+      [set_solver
+      |set_solver
+      |(destruct (uses_kt pf1),(uses_kt pf2); simpl in *; congruence)
+      |idtac]
+    .
+    unfold is_true in pwi_pf_kt.
+    rewrite implb_true_iff in pwi_pf_kt.
+    unfold is_true in pwi_pf_kta.
+    rewrite implb_true_iff in pwi_pf_kta.
+    unfold is_true in pwi_pf_kt0.
+    rewrite implb_true_iff in pwi_pf_kt0.
+    unfold is_true in pwi_pf_kta0.
+    rewrite implb_true_iff in pwi_pf_kta0.
+    unfold is_true.
+    rewrite implb_true_iff.
+    intro H.
+    rewrite orb_true_iff in H.
+    destruct H as [H|H].
+    {
+      specialize (pwi_pf_kta H).
+      rewrite andb_true_iff in pwi_pf_kta.
+      destruct pwi_pf_kta as [H1 H2].
+      rewrite H1 H2. reflexivity.
+    }
+    {
+      specialize (pwi_pf_kta0 H).
+      rewrite andb_true_iff in pwi_pf_kta0.
+      destruct pwi_pf_kta0 as [H1 H2].
+      rewrite H1 H2.
+      rewrite orb_true_r.
+      reflexivity.
+    }
   }
 Defined.
 
@@ -149,72 +183,6 @@ Defined.
     exact _5.
   Defined.
 
-  Lemma ProofLe_ProofInfoLe {Σ : Signature} i₁ i₂:
-    ProofLe i₁ i₂ ->
-    ProofInfoLe i₁ i₂.
-  Proof.
-    intros pile. destruct i₁, i₂.
-    repeat split.
-    {
-      unfold ProofLe in pile.
-      rewrite elem_of_subseteq.
-      intros x Hx.
-      remember (fresh_evar (patt_free_evar x)) as y.
-      pose (pf1 := A_impl_A ∅ (patt_free_evar y) ltac:(wf_auto2)).
-      pose (pf2 := ProofSystem.Ex_gen ∅ (patt_free_evar y) (patt_free_evar y) x ltac:(wf_auto2) ltac:(wf_auto2) (proj1_sig pf1) ltac:(simpl; rewrite elem_of_singleton; solve_fresh_neq)).
-      specialize (pile ∅ _ pf2).
-      feed specialize pile.
-      {
-        constructor.
-        { simpl. clear -Hx. set_solver. }
-        { simpl. clear. set_solver. }
-        { simpl. reflexivity. }
-      }
-      destruct pile as [Hm2 Hm3 Hm4].
-      simpl in *.
-      clear -Hm2.
-      set_solver.
-    }
-    {
-      unfold ProofLe in pile.
-      rewrite elem_of_subseteq.
-      intros X HX.
-      pose (pf1 := A_impl_A ∅ (patt_free_svar X) ltac:(wf_auto2)).
-      pose (pf2 := ProofSystem.Svar_subst ∅ (patt_free_svar X ---> patt_free_svar X) patt_bott X ltac:(wf_auto2) ltac:(wf_auto2) (proj1_sig pf1)).
-      specialize (pile ∅ _ pf2).
-      feed specialize pile.
-      {
-        constructor; simpl.
-        { clear. set_solver. }
-        { clear -HX. set_solver. }
-        { reflexivity. }
-      }
-      destruct pile as [Hp2 Hp3 Hp4].
-      simpl in *.
-      clear -Hp3.
-      set_solver.
-    }
-    {
-      unfold ProofLe in pile.
-      pose (pf1 := A_impl_A ∅ patt_bott ltac:(wf_auto2)).
-      pose (pf2 := ProofSystem.Knaster_tarski ∅ (patt_bound_svar 0) patt_bott ltac:(wf_auto2) (proj1_sig pf1)).
-      destruct pi_uses_kt.
-      2: { simpl. reflexivity. }
-      specialize (pile ∅ _ pf2).
-      feed specialize pile.
-      {
-        constructor; simpl.
-        { clear. set_solver. }
-        { clear. set_solver. }
-        { reflexivity. }
-      }
-      destruct pile as [Hp2 Hp3 Hp4].
-      simpl in Hp4.
-      rewrite Hp4.
-      reflexivity.
-    }
-  Qed.
-
 Lemma useGenericReasoning  {Σ : Signature} (Γ : Theory) (ϕ : Pattern) i' i:
   (ProofInfoLe i' i) ->
   Γ ⊢i ϕ using i' ->
@@ -223,7 +191,7 @@ Proof.
   intros pile [pf Hpf].
   exists pf.
 
-  destruct Hpf as [Hpf2 Hpf3 Hpf4].
+  destruct Hpf as [Hpf2 Hpf3 Hpf4 Hpf5].
   destruct i, i'; cbn in *.
   destruct pile as [H [H0 H1] ].
   constructor; simpl.
@@ -232,6 +200,15 @@ Proof.
   { simpl in *. apply implb_true_iff.
     unfold is_true in *. rewrite implb_true_iff in Hpf4 H1.
     set_solver.
+  }
+  {
+    simpl in *. apply implb_true_iff.
+    unfold is_true in *. rewrite implb_true_iff in Hpf5 H1.
+    destruct H1 as [H11 H12].
+    rewrite implb_true_iff in H11.
+    rewrite implb_true_iff in H12.
+    intros H'.
+    naive_solver.
   }
 Defined.
 
@@ -347,7 +324,7 @@ Proof.
 Defined.
 
 Lemma pile_impl_allows_gen_x {Σ : Signature} x gpi svs kt:
-  ProofInfoLe ( (ExGen := {[x]}, SVSubst := svs, KT := kt)) ( gpi) ->
+  ProofInfoLe ( (ExGen := {[x]}, SVSubst := svs, KT := kt, AKT := false)) ( gpi) ->
   x ∈ pi_generalized_evars gpi.
 Proof.
   destruct gpi. intro H.
@@ -355,7 +332,7 @@ Proof.
 Qed.
 
 Lemma pile_impl_uses_kt {Σ : Signature} gpi evs svs:
-  ProofInfoLe ( (ExGen := evs, SVSubst := svs, KT := true)) ( gpi) ->
+  ProofInfoLe ( (ExGen := evs, SVSubst := svs, KT := true, AKT := false)) ( gpi) ->
   pi_uses_kt gpi.
 Proof.
   destruct gpi. intro H.
@@ -363,7 +340,7 @@ Proof.
 Qed.
 
 Lemma pile_impl_allows_svsubst_X {Σ : Signature} gpi evs X kt:
-  ProofInfoLe ( (ExGen := evs, SVSubst := {[X]}, KT := kt)) ( gpi) ->
+  ProofInfoLe ( (ExGen := evs, SVSubst := {[X]}, KT := kt, AKT := false)) ( gpi) ->
   X ∈ pi_substituted_svars gpi.
 Proof.
   destruct gpi. intro H.
